

## Strain component $\varepsilon_{xx}$ for an edge dislocation

The displacement field is

$$u_x = \frac{b}{2\pi} \left[ \tan^{-1}\left(\frac{y}{x}\right) + \frac{xy}{2(1-\nu)(x^2+y^2)} \right].$$

Thus,

$$\varepsilon_{xx} = \frac{\partial u_x}{\partial x} = \frac{b}{2\pi} \left[ \frac{\partial}{\partial x} \tan^{-1}\left(\frac{y}{x}\right) + \frac{\partial}{\partial x} \left( \frac{xy}{2(1-\nu)(x^2+y^2)} \right) \right].$$

### Derivative of the first term

$$\frac{\partial}{\partial x} \tan^{-1}\left(\frac{y}{x}\right) = \frac{1}{1+(y/x)^2} \left(-\frac{y}{x^2}\right) = -\frac{y}{x^2+y^2}.$$

### Derivative of the second term

$$\frac{\partial}{\partial x} \left( \frac{xy}{x^2+y^2} \right) = \frac{y(x^2+y^2) - xy(2x)}{(x^2+y^2)^2} = \frac{y(y^2-x^2)}{(x^2+y^2)^2}.$$

Including the constant factor:

$$\frac{\partial}{\partial x} \left( \frac{xy}{2(1-\nu)(x^2+y^2)} \right) = \frac{y(y^2-x^2)}{2(1-\nu)(x^2+y^2)^2}.$$

### Combine both parts

$$\varepsilon_{xx} = \frac{b}{2\pi} \left[ -\frac{y}{x^2+y^2} + \frac{y(y^2-x^2)}{2(1-\nu)(x^2+y^2)^2} \right].$$

### Convert to polar coordinates

Using

$$x = r \cos \theta, \quad y = r \sin \theta, \quad x^2 + y^2 = r^2, \quad y^2 - x^2 = -r^2 \cos 2\theta,$$

we obtain

$$\begin{aligned} -\frac{y}{x^2+y^2} &= -\frac{r \sin \theta}{r^2} = -\frac{\sin \theta}{r}, \\ \frac{y(y^2-x^2)}{2(1-\nu)(x^2+y^2)^2} &= \frac{r \sin \theta (-r^2 \cos 2\theta)}{2(1-\nu)r^4} = -\frac{\sin \theta \cos 2\theta}{2(1-\nu)r}. \end{aligned}$$

### Final expression

$$\boxed{\varepsilon_{xx} = -\frac{b}{2\pi r} \left[ \sin \theta + \frac{\sin \theta \cos 2\theta}{2(1-\nu)} \right].}$$

## Strain component $\varepsilon_{yy}$ for an edge dislocation

The displacement field is

$$u_y = -\frac{b}{2\pi} \left[ \frac{1-2\nu}{4(1-\nu)} \ln(x^2 + y^2) + \frac{x^2 - y^2}{4(1-\nu)(x^2 + y^2)} \right].$$

Hence,

$$\varepsilon_{yy} = \frac{\partial u_y}{\partial y} = -\frac{b}{2\pi} \left[ \frac{1-2\nu}{4(1-\nu)} \frac{\partial}{\partial y} \ln(x^2 + y^2) + \frac{\partial}{\partial y} \left( \frac{x^2 - y^2}{4(1-\nu)(x^2 + y^2)} \right) \right].$$

### Derivative of the first term

$$\frac{\partial}{\partial y} \ln(x^2 + y^2) = \frac{2y}{x^2 + y^2}.$$

### Derivative of the second term

Using the quotient rule,

$$\frac{\partial}{\partial y} \left( \frac{x^2 - y^2}{x^2 + y^2} \right) = \frac{-2y(x^2 + y^2) - (x^2 - y^2)(2y)}{(x^2 + y^2)^2} = \frac{-4x^2y}{(x^2 + y^2)^2}.$$

Including the constant,

$$\frac{\partial}{\partial y} \left( \frac{x^2 - y^2}{4(1-\nu)(x^2 + y^2)} \right) = \frac{-x^2y}{(1-\nu)(x^2 + y^2)^2}.$$

### Combine both contributions

$$\varepsilon_{yy} = -\frac{b}{2\pi} \left[ \frac{1-2\nu}{4(1-\nu)} \frac{2y}{x^2 + y^2} - \frac{x^2y}{(1-\nu)(x^2 + y^2)^2} \right].$$

### Convert to polar form

$$x = r \cos \theta, \quad y = r \sin \theta, \quad x^2 + y^2 = r^2.$$

Thus,

$$\begin{aligned} \frac{2y}{x^2 + y^2} &= \frac{2r \sin \theta}{r^2} = \frac{2 \sin \theta}{r}, \\ \frac{-x^2y}{(x^2 + y^2)^2} &= \frac{-r^2 \cos^2 \theta r \sin \theta}{r^4} = -\frac{\cos^2 \theta \sin \theta}{r}. \end{aligned}$$

### Final expression

$$\boxed{\varepsilon_{yy} = -\frac{b}{2\pi r} \left[ \frac{1-2\nu}{2(1-\nu)} \sin \theta - \frac{\cos^2 \theta \sin \theta}{1-\nu} \right]}$$

## Strain component $\varepsilon_{xy}$ for an edge dislocation

The displacement fields are

$$u_x = \frac{b}{2\pi} \left[ \tan^{-1}\left(\frac{y}{x}\right) + \frac{xy}{2(1-\nu)(x^2+y^2)} \right],$$
$$u_y = -\frac{b}{2\pi} \left[ \frac{1-2\nu}{4(1-\nu)} \ln(x^2+y^2) + \frac{x^2-y^2}{4(1-\nu)(x^2+y^2)} \right].$$

The engineering shear strain is

$$\varepsilon_{xy} = \frac{1}{2} \left( \frac{\partial u_x}{\partial y} + \frac{\partial u_y}{\partial x} \right).$$

### Derivative of $u_x$ with respect to $y$

$$\frac{\partial}{\partial y} \tan^{-1}\left(\frac{y}{x}\right) = \frac{x}{x^2+y^2},$$
$$\frac{\partial}{\partial y} \left( \frac{xy}{x^2+y^2} \right) = \frac{x(x^2-y^2)}{(x^2+y^2)^2}.$$

Including constants:

$$\frac{\partial}{\partial y} \left( \frac{xy}{2(1-\nu)(x^2+y^2)} \right) = \frac{x(x^2-y^2)}{2(1-\nu)(x^2+y^2)^2}.$$

Thus,

$$\frac{\partial u_x}{\partial y} = \frac{b}{2\pi} \left[ \frac{x}{x^2+y^2} + \frac{x(x^2-y^2)}{2(1-\nu)(x^2+y^2)^2} \right].$$

### Derivative of $u_y$ with respect to $x$

$$\frac{\partial}{\partial x} \ln(x^2+y^2) = \frac{2x}{x^2+y^2},$$
$$\frac{\partial}{\partial x} \left( \frac{x^2-y^2}{x^2+y^2} \right) = \frac{4xy^2}{(x^2+y^2)^2}.$$

Including constants:

$$\frac{\partial}{\partial x} \left( \frac{x^2-y^2}{4(1-\nu)(x^2+y^2)} \right) = \frac{xy^2}{(1-\nu)(x^2+y^2)^2}.$$

Thus,

$$\frac{\partial u_y}{\partial x} = -\frac{b}{2\pi} \left[ \frac{1-2\nu}{4(1-\nu)} \frac{2x}{x^2+y^2} + \frac{xy^2}{(1-\nu)(x^2+y^2)^2} \right].$$

### Combine contributions

$$\varepsilon_{xy} = \frac{1}{2} \left( \frac{b}{2\pi} \left[ \frac{x}{x^2 + y^2} + \frac{x(x^2 - y^2)}{2(1 - \nu)(x^2 + y^2)^2} \right] - \frac{b}{2\pi} \left[ \frac{1 - 2\nu}{2(1 - \nu)} \frac{x}{x^2 + y^2} + \frac{xy^2}{(1 - \nu)(x^2 + y^2)^2} \right] \right).$$

### Convert to polar form

$$x = r \cos \theta, \quad x^2 - y^2 = r^2 \cos 2\theta, \quad xy^2 = r^3 \cos \theta \sin^2 \theta.$$

Then

$$\begin{aligned} \frac{x}{x^2 + y^2} &= \frac{\cos \theta}{r}, & \frac{x(x^2 - y^2)}{2(1 - \nu)(x^2 + y^2)^2} &= \frac{\cos \theta \cos 2\theta}{2(1 - \nu)r}, \\ \frac{2x}{x^2 + y^2} &= \frac{2 \cos \theta}{r}, & \frac{xy^2}{(x^2 + y^2)^2} &= \frac{\cos \theta \sin^2 \theta}{r}. \end{aligned}$$

### Final expression

$$\boxed{\varepsilon_{xy} = \frac{b}{4\pi r} \left[ \cos \theta + \frac{\cos \theta \cos 2\theta}{2(1 - \nu)} - \frac{1 - 2\nu}{2(1 - \nu)} \cos \theta - \frac{\cos \theta \sin^2 \theta}{1 - \nu} \right]}.$$

$$\boxed{\varepsilon_{xy} = \frac{b}{4\pi r(1 - \nu)} \cos \theta \cos 2\theta}$$

## Stress Components from Strain Fields (Plane Strain)

### Strain fields

$$\begin{aligned}\varepsilon_{xx} &= -\frac{b}{2\pi r} \left[ \sin \theta + \frac{\sin \theta \cos 2\theta}{2(1-\nu)} \right], \\ \varepsilon_{yy} &= -\frac{b}{2\pi r} \left[ \frac{1}{2(1-\nu)} \sin \theta - \frac{\sin \theta \cos 2\theta}{2(1-\nu)} \right], \\ \varepsilon_{xy} &= \frac{b}{4\pi r(1-\nu)} \cos \theta \cos 2\theta.\end{aligned}$$

### Hooke's law (plane strain)

$$\begin{aligned}\sigma_{xx} &= 2G\varepsilon_{xx} + \lambda(\varepsilon_{xx} + \varepsilon_{yy}), & \sigma_{yy} &= 2G\varepsilon_{yy} + \lambda(\varepsilon_{xx} + \varepsilon_{yy}), \\ \sigma_{xy} &= 2G\varepsilon_{xy}.\end{aligned}$$

$$G = \frac{E}{2(1+\nu)}, \quad \lambda = \frac{2G\nu}{1-2\nu}.$$

### Trace term

$$\varepsilon_{xx} + \varepsilon_{yy} = -\frac{b}{2\pi r} \frac{\sin \theta}{1-\nu}.$$

### Stress component $\sigma_{yy}$

$$\begin{aligned}\sigma_{yy} &= 2G\varepsilon_{yy} + \lambda(\varepsilon_{xx} + \varepsilon_{yy}), \\ \sigma_{yy} &= -\frac{b}{2\pi r} \left[ 2G \left( \frac{\sin \theta - \sin \theta \cos 2\theta}{2(1-\nu)} \right) + \lambda \left( \frac{\sin \theta}{1-\nu} \right) \right].\end{aligned}$$

Factor common terms:

$$\sigma_{yy} = -\frac{b}{2\pi r} \frac{\sin \theta}{1-\nu} [G(1 - \cos 2\theta) + \lambda].$$

Use  $1 - \cos 2\theta = 2 \sin^2 \theta$ :

$$\sigma_{yy} = -\frac{b}{2\pi r} \frac{\sin \theta}{1-\nu} [2G \sin^2 \theta + \lambda].$$

Substitute  $\lambda = \frac{2G\nu}{1-2\nu}$ :

$$\boxed{\sigma_{yy} = -\frac{Gb}{2\pi r(1-\nu)} \sin \theta \left( 2 \sin^2 \theta + \frac{2\nu}{1-2\nu} \right)}.$$

**Stress component  $\sigma_{xy}$**

$$\sigma_{xy} = 2G \varepsilon_{xy} = 2G \left[ \frac{b}{4\pi r(1-\nu)} \cos \theta \cos 2\theta \right],$$

Simplified:

$$\boxed{\sigma_{xy} = \frac{Gb}{2\pi r(1-\nu)} \cos \theta \cos 2\theta.}$$

**Stress Field of an Edge Dislocation in Terms of Shear Modulus  $G$**

$$\sigma_{xx} = -\frac{Gb}{2\pi(1-\nu)} \frac{\sin \theta}{r} [1 - \cos 2\theta],$$

$$\sigma_{yy} = -\frac{Gb}{2\pi(1-\nu)} \frac{\sin \theta}{r} [1 + \cos 2\theta],$$

$$\sigma_{xy} = \frac{Gb}{2\pi(1-\nu)} \frac{\cos \theta \cos 2\theta}{r}.$$